typeArith/ocaml/src/lexer.mll
@@ -1,0 +1,22 @@
+{
+  exception Error of string
+}
+
+rule main = parse
+  (* ignore spacing and newline characters *)
+  [' ' '\009' '\012' '\n']+     { main lexbuf }
+| "("   { Parser.LPAREN }
+| ")"   { Parser.RPAREN }
+| ";"   { Parser.SEMI }
+| "O"   { Parser.ZERO }
+| "S"   { Parser.SUCC }
+| "Pred"{ Parser.PRED }
+| "if"  { Parser.IF }
+| "is0" {Parser.ISO}
+| "else"{ Parser.ELSE }
+| "then"{ Parser.THEN }
+|"tru"  { Parser.TRUE }
+|"fls"  { Parser.FALSE }
+| eof   { exit 0 }
+| _     { raise (Error (Printf.sprintf "At offset %d: unexpected character." (Lexing.lexeme_start lexbuf))) }
+
