typeArith/ocaml/src/print.ml
@@ -1,0 +1,18 @@
+open Eval
+
+let rec eval_string t =
+  match t with
+  | Tru -> "Tru"
+  | Fls -> "Fls"
+  | If (t1, t2, t3) -> "If " ^ (eval_string t1) ^ " THEN " ^ (eval_string t2) ^ " ELSE " ^ (eval_string t3)
+  | O   -> "0"
+  | Succ t1 -> "S (" ^ (eval_string t1) ^ ")"
+  | Pred t1 -> "Pred " ^ (eval_string t1)
+  | Iszero t1 -> "Is0 " ^ (eval_string t1)
+
+
+let rec manyeval t1 =
+  match eval t1 with
+  | Some t1' -> manyeval t1'
+  | _        -> t1
+
